silveroak-opentitan/aes/Spec/ExpandAllKeys.v
@@ -1,3 +1,4 @@
+(****************************************************************************)
 (* Copyright 2020 The Project Oak Authors                                   *)
 (*                                                                          *)
 (* Licensed under the Apache License, Version 2.0 (the "License")           *)
@@ -106,3 +107,82 @@ Section Spec.
     Qed.
   End Properties.
 End Spec.
+
+Section Inverse.
+  Context {key : Type}.
+
+  Lemma all_keys'_inv_eq :
+    forall (key_expand inv_key_expand : nat -> key -> key)
+      round_idxs initial_key final_key
+      (final_key_correct :
+         snd (all_keys' key_expand round_idxs initial_key) = final_key)
+      (inv_key_expand_key_expand :
+         forall i k,
+           inv_key_expand i (key_expand i k) = k),
+      fst (all_keys' inv_key_expand (rev round_idxs) final_key)
+      = rev (fst (all_keys' key_expand round_idxs initial_key)).
+  Proof.
+    cbv [all_keys'].
+    induction round_idxs using rev_ind; intros;
+      autorewrite with listsimpl; cbn [rev app];
+        autorewrite with push_fold_acc.
+    { rewrite @fold_left_accumulate_snd in *.
+      cbn [fold_left rev app] in *. congruence. }
+    { rewrite !fold_left_accumulate_snoc. cbv zeta.
+      autorewrite with listsimpl in *. cbn [rev app] in *.
+      rewrite @fold_left_accumulate_snd in *.
+      rewrite fold_left_app in final_key_correct.
+      cbn [fold_left] in *. rewrite <-final_key_correct.
+      erewrite <-IHround_idxs; [ reflexivity | | assumption ].
+      rewrite fold_left_accumulate_snd.
+      rewrite inv_key_expand_key_expand.
+      reflexivity. }
+  Qed.
+
+  Lemma all_keys'_rev_seq :
+    forall n (kexpand kexpand_rev : nat -> key -> key) (initial_key : key)
+      (Hequiv : forall i k, kexpand_rev i k = kexpand (n - S i) k),
+      fst (all_keys' kexpand (seq 0 n) initial_key)
+      = fst (all_keys' kexpand_rev (rev (seq 0 n)) initial_key).
+  Proof.
+    cbv [all_keys'].
+    induction n; intros; [ reflexivity | ].
+    rewrite rev_seq_S, Nat.add_0_l. cbn [seq].
+    autorewrite with push_fold_acc.
+    rewrite <-seq_shift, fold_left_accumulate_map.
+    erewrite IHn by (intros; instantiate_app_by_reflexivity).
+    rewrite Hequiv, Nat.sub_diag.
+    erewrite fold_left_accumulate_ext1_In; [ reflexivity | ].
+    intros *. rewrite in_rev, rev_involutive, in_seq.
+    intros; cbv beta; rewrite Hequiv.
+    f_equal; lia.
+  Qed.
+
+  Lemma last_all_keys (key_expand : nat -> key -> key) k :
+    forall Nr initial_key,
+      last (all_keys key_expand Nr initial_key) k =
+      snd (all_keys' key_expand (seq 0 Nr) initial_key).
+  Proof.
+    cbv [all_keys all_keys']; intros.
+    rewrite fold_left_accumulate_last, fold_left_accumulate_snd.
+    reflexivity.
+  Qed.
+
+  Lemma all_keys_inv_eq (key_expand inv_key_expand : nat -> key -> key) :
+    forall Nr initial_key final_key
+      (final_key_correct :
+         forall k, last (all_keys key_expand Nr initial_key) k = final_key)
+      (inv_key_expand_key_expand :
+         forall i k, inv_key_expand (Nr - S i) (key_expand i k) = k),
+    all_keys inv_key_expand Nr final_key
+    = rev (all_keys key_expand Nr initial_key).
+  Proof.
+    intros; cbv [all_keys].
+    erewrite <-all_keys'_inv_eq
+      with (inv_key_expand:=fun i => inv_key_expand (Nr - S i))  by eauto.
+    erewrite all_keys'_rev_seq by (intros; instantiate_app_by_reflexivity).
+    erewrite <-(final_key_correct initial_key), last_all_keys.
+    reflexivity.
+  Qed.
+
+End Inverse.
